PiLL/Model/Judgement.lean
@@ -130,8 +130,6 @@ def proc {𝒢 : HyperEnv} {P : Proc} {n : Nat} (_ : n ⊢ P ∷ 𝒢) : Proc :=
 def env {𝒢 : HyperEnv} {P : Proc} {n : Nat} (_ : n ⊢ P ∷ 𝒢) : HyperEnv := 𝒢
 
 
-
-
 -- FIXME: Get these working again
 -- lemma Typing.env_comm {P : Proc} {𝒢 : HyperEnv} {Γ Δ : Env} :
 --   (⊢ P ∷ 𝒢 |ₕ Γ‚ Δ) → (⊢ P ∷ 𝒢 |ₕ Δ‚ Γ) :=
